internal/examples/semantics/multiple_return.go
@@ -1,0 +1,24 @@
+package semantics
+
+func returnTwo() (uint64, uint64) {
+	return 2, 3
+}
+
+func testReturnTwo() bool {
+	x, y := returnTwo()
+	return x == 2 && y == 3
+}
+
+func testAnonymousBinding() bool {
+	_, y := returnTwo()
+	return y == 3
+}
+
+func returnThree() (uint64, bool, uint32) {
+	return 2, true, 1
+}
+
+func failing_testReturnThree() bool {
+	x, y, z := returnThree()
+	return x == 2 && y == true && z == 1
+}
